#### Equazione

$$(1+x)^{n} \geq 1 + nx \quad \forall n \in \mathbb{N} , \quad \forall x \in \mathbb{R} : x> -1$$
#### Dimostrazione per [[Principio di induzione|induzione]]

Passo 1 per n = 0:
$$n=0 \rightarrow (1+x)^{0} \geq 1+0 \cdot x \rightarrow 1 \geq 1$$
Ipotesi:
$$(1+x)^{n} \geq 1 + nx$$
tesi:
$$(1+x)^{n+1} \geq 1+(n+1)x$$
Dim:
$$(1+x)^{n} \cdot (1+x) \geq (1+nx) \cdot (1+x)$$
$$\rightarrow (1+x)^{n+1} \geq 1 + x + nx + nx^{2}$$
Ma sappiamo che le c.e. $\forall n \in \mathbb{N} \quad \forall x \in \mathbb{R} : x > -1$
quindi: 
$$nx^{2} > 0$$
quindi Ã¨ dimostrato.
